Substitute interpretations of store rels and bit exprs.

deps/poulet4/lib/P4automata/ConfRel.v
@@ -98,6 +98,9 @@ Section ConfRel.
     { st_state: state_ref (P4A.interp a);
       st_buf_len: nat }.
 
+  Definition state_template_sane (st: state_template) :=
+    st.(st_buf_len) < size' (P4A.interp a) st.(st_state).
+
   Global Program Instance state_template_eq_dec : EquivDec.EqDec state_template eq :=
     { equiv_dec x y :=
         if x.(st_state) == y.(st_state)
@@ -223,45 +226,21 @@ Section ConfRel.
       be_size b1 b2 e1 + be_size b1 b2 e2
     end.
 
-  Equations interp_bit_expr {c} (e: bit_expr c) (valu: bval c) (c1 c2: conf)
-    : n_tuple bool (be_size (conf_buf_len c1) (conf_buf_len c2) e) := {
-    interp_bit_expr (BELit l) valu c1 c2 :=
+  Equations interp_bit_expr {b1 b2 c}
+    (e: bit_expr c)
+    (valu: bval c)
+    (buf1: n_tuple bool b1)
+    (buf2: n_tuple bool b2)
+    (store1 store2: store (P4A.interp a))
+    : n_tuple bool (be_size b1 b2 e)
+  := {
+    interp_bit_expr (BELit l) valu buf1 buf2 store1 store2 :=
       l2t l;
-    interp_bit_expr (BEBuf Left) valu c1 c2 :=
-      conf_buf c1;
-    interp_bit_expr (BEBuf Right) valu c1 c2 :=
-      conf_buf c2;
-    interp_bit_expr (BEHdr a h) valu c1 c2 :=
-      let c := match a with
-               | Left => c1
-               | Right => c2
-               end
-      in
-      match h with
-      | P4A.HRVar var =>
-        match P4A.find H (projT2 var) (conf_store c)  with
-        | P4A.VBits _ v => v
-        end
-      end;
-    interp_bit_expr (BEVar x) valu c1 c2 :=
-      interp_bvar valu x;
-    interp_bit_expr (BESlice e hi lo) valu c1 c2 :=
-      n_tuple_slice hi lo (interp_bit_expr e valu c1 c2);
-    interp_bit_expr (BEConcat e1 e2) valu c1 c2 :=
-      n_tuple_concat
-        (interp_bit_expr e1 valu c1 c2)
-        (interp_bit_expr e2 valu c1 c2)
-  }.
-
-  Equations interp_simplified_bit_expr {b1 b2 c} (e: bit_expr c) (valu: bval c) (buf1: n_tuple bool b1) (buf2: n_tuple bool b2) (store1 store2: store (P4A.interp a))
-    : n_tuple bool (be_size b1 b2 e) := {
-    interp_simplified_bit_expr (BELit l) valu buf1 buf2 store1 store2 :=
-      l2t l;
-    interp_simplified_bit_expr (BEBuf Left) valu buf1 buf2 store1 store2 :=
+    interp_bit_expr (BEBuf Left) valu buf1 buf2 store1 store2 :=
       buf1;
-    interp_simplified_bit_expr (BEBuf Right) valu buf1 buf2 store1 store2 :=
+    interp_bit_expr (BEBuf Right) valu buf1 buf2 store1 store2 :=
       buf2;
-    interp_simplified_bit_expr (BEHdr a h) valu buf1 buf2 store1 store2 :=
+    interp_bit_expr (BEHdr a h) valu buf1 buf2 store1 store2 :=
       let store := match a with
                | Left => store1
                | Right => store2
@@ -273,26 +252,15 @@ Section ConfRel.
         | P4A.VBits _ v => v
         end
       end;
-    interp_simplified_bit_expr (BEVar x) valu buf1 buf2 store1 store2 :=
+    interp_bit_expr (BEVar x) valu buf1 buf2 store1 store2 :=
       interp_bvar valu x;
-    interp_simplified_bit_expr (BESlice e hi lo) valu buf1 buf2 store1 store2 :=
-      n_tuple_slice hi lo (interp_simplified_bit_expr e valu buf1 buf2 store1 store2);
-    interp_simplified_bit_expr (BEConcat e1 e2) valu buf1 buf2 store1 store2 :=
+    interp_bit_expr (BESlice e hi lo) valu buf1 buf2 store1 store2 :=
+      n_tuple_slice hi lo (interp_bit_expr e valu buf1 buf2 store1 store2);
+    interp_bit_expr (BEConcat e1 e2) valu buf1 buf2 store1 store2 :=
       n_tuple_concat
-        (interp_simplified_bit_expr e1 valu buf1 buf2 store1 store2)
-        (interp_simplified_bit_expr e2 valu buf1 buf2 store1 store2)
+        (interp_bit_expr e1 valu buf1 buf2 store1 store2)
+        (interp_bit_expr e2 valu buf1 buf2 store1 store2)
   }.
-
-  Lemma interp_bit_expr_simplify c (e: bit_expr c) (valu: bval c) (c1 c2: conf):
-    interp_bit_expr e valu c1 c2 =
-    interp_simplified_bit_expr e valu c1.(conf_buf) c2.(conf_buf) c1.(conf_store) c2.(conf_store).
-  Proof.
-    induction e;
-    try destruct a0;
-    autorewrite with interp_bit_expr;
-    autorewrite with interp_simplified_bit_expr;
-    reflexivity || congruence.
-  Qed.
 
   Inductive store_rel c :=
   | BRTrue
@@ -392,94 +360,64 @@ Section ConfRel.
     | BRImpl r1 r2 => BRImpl (weaken_store_rel size r1) (weaken_store_rel size r2)
     end.
 
-  Equations interp_store_rel {c} (r: store_rel c) (valu: bval c) (c1 c2: conf) : Prop := {
-    interp_store_rel (BRTrue _) valu c1 c2 :=
-      True;
-    interp_store_rel (BRFalse _) valu c1 c2 :=
-      False;
-    interp_store_rel (BREq e1 e2) valu c1 c2 :=
-      match eq_dec (be_size (conf_buf_len c1) (conf_buf_len c2) e1)
-                   (be_size (conf_buf_len c1) (conf_buf_len c2) e2) with
-      | left Heq =>
-        eq_rect _ _ (interp_bit_expr e1 valu c1 c2) _ Heq =
-        interp_bit_expr e2 valu c1 c2
-      | right _ => False
-      end;
-    interp_store_rel (BRAnd r1 r2) valu c1 c2 :=
-      interp_store_rel r1 valu c1 c2 /\ interp_store_rel r2 valu c1 c2;
-    interp_store_rel (BROr r1 r2) valu c1 c2 :=
-      interp_store_rel r1 valu c1 c2 \/ interp_store_rel r2 valu c1 c2;
-    interp_store_rel (BRImpl r1 r2) valu c1 c2 :=
-      interp_store_rel r1 valu c1 c2 -> interp_store_rel r2 valu c1 c2
-  }.
-
-  Equations interp_simplified_store_rel {b1 b2 c}
+  Equations interp_store_rel {b1 b2 c}
     (r: store_rel c)
     (valu: bval c)
     (buf1: n_tuple bool b1)
     (buf2: n_tuple bool b2)
     (store1 store2: store (P4A.interp a))
     : Prop := {
-    interp_simplified_store_rel (BRTrue _) valu buf1 buf2 store1 store2 :=
+    interp_store_rel (BRTrue _) valu buf1 buf2 store1 store2 :=
       True;
-    interp_simplified_store_rel (BRFalse _) valu buf1 buf2 store1 store2 :=
+    interp_store_rel (BRFalse _) valu buf1 buf2 store1 store2 :=
       False;
-    interp_simplified_store_rel (BREq e1 e2) valu buf1 buf2 store1 store2 :=
+    interp_store_rel (BREq e1 e2) valu buf1 buf2 store1 store2 :=
       match eq_dec (be_size b1 b2 e1) (be_size b1 b2 e2) with
       | left Heq =>
-        eq_rect _ _ (interp_simplified_bit_expr e1 valu buf1 buf2 store1 store2) _ Heq =
-        interp_simplified_bit_expr e2 valu buf1 buf2 store1 store2
+        eq_rect _ _ (interp_bit_expr e1 valu buf1 buf2 store1 store2) _ Heq =
+        interp_bit_expr e2 valu buf1 buf2 store1 store2
       | right _ => False
       end;
-    interp_simplified_store_rel (BRAnd r1 r2) valu buf1 buf2 store1 store2 :=
-      interp_simplified_store_rel r1 valu buf1 buf2 store1 store2 /\
-      interp_simplified_store_rel r2 valu buf1 buf2 store1 store2;
-    interp_simplified_store_rel (BROr r1 r2) valu buf1 buf2 store1 store2 :=
-      interp_simplified_store_rel r1 valu buf1 buf2 store1 store2 \/
-      interp_simplified_store_rel r2 valu buf1 buf2 store1 store2;
-    interp_simplified_store_rel (BRImpl r1 r2) valu buf1 buf2 store1 store2 :=
-      interp_simplified_store_rel r1 valu buf1 buf2 store1 store2 ->
-      interp_simplified_store_rel r2 valu buf1 buf2 store1 store2
+    interp_store_rel (BRAnd r1 r2) valu buf1 buf2 store1 store2 :=
+      interp_store_rel r1 valu buf1 buf2 store1 store2 /\
+      interp_store_rel r2 valu buf1 buf2 store1 store2;
+    interp_store_rel (BROr r1 r2) valu buf1 buf2 store1 store2 :=
+      interp_store_rel r1 valu buf1 buf2 store1 store2 \/
+      interp_store_rel r2 valu buf1 buf2 store1 store2;
+    interp_store_rel (BRImpl r1 r2) valu buf1 buf2 store1 store2 :=
+      interp_store_rel r1 valu buf1 buf2 store1 store2 ->
+      interp_store_rel r2 valu buf1 buf2 store1 store2
   }.
-
-  Lemma interp_store_rel_simplify c (sr: store_rel c) (valu: bval c) (c1 c2: conf):
-    interp_store_rel sr valu c1 c2 <->
-    interp_simplified_store_rel sr valu c1.(conf_buf)
-                                        c2.(conf_buf)
-                                        c1.(conf_store)
-                                        c2.(conf_store).
-  Proof.
-    revert sr valu c1 c2; induction sr; intros;
-    autorewrite with interp_store_rel;
-    autorewrite with interp_simplified_store_rel;
-    try tauto.
-    - destruct (eq_dec _ _); try reflexivity.
-      now repeat rewrite interp_bit_expr_simplify.
-    - intuition.
-    - intuition.
-    - intuition.
-  Qed.
 
   (* correctness of smart constructors *)
   Lemma bror_corr :
-    forall c (l r: store_rel c) v c1 c2,
-        interp_store_rel (BROr l r) v c1 c2 <-> interp_store_rel (bror l r) v c1 c2.
+    forall c (l r: store_rel c) v
+           b1 b2 (buf1: n_tuple bool b1) (buf2: n_tuple bool b2)
+           store1 store2,
+        interp_store_rel (BROr l r) v buf1 buf2 store1 store2 <->
+        interp_store_rel (bror l r) v buf1 buf2 store1 store2.
   Proof.
     split; intros; destruct l, r; unfold bror in *;
     autorewrite with interp_store_rel in *; auto; intuition.
   Qed.
 
   Lemma brand_corr :
-    forall c (l r: store_rel c) v c1 c2,
-        interp_store_rel (BRAnd l r) v c1 c2 <-> interp_store_rel (brand l r) v c1 c2.
+    forall c (l r: store_rel c) v
+           b1 b2 (buf1: n_tuple bool b1) (buf2: n_tuple bool b2)
+           store1 store2,
+        interp_store_rel (BRAnd l r) v buf1 buf2 store1 store2 <->
+        interp_store_rel (brand l r) v buf1 buf2 store1 store2.
   Proof.
     split; intros; destruct l, r; unfold brand in *;
     autorewrite with interp_store_rel in *; auto; intuition.
   Qed.
 
   Lemma brimpl_corr :
-    forall c (l r: store_rel c) v c1 c2,
-        interp_store_rel (BRImpl l r) v c1 c2 <-> interp_store_rel (brimpl l r) v c1 c2.
+    forall c (l r: store_rel c) v
+           b1 b2 (buf1: n_tuple bool b1) (buf2: n_tuple bool b2)
+           store1 store2,
+        interp_store_rel (BRImpl l r) v buf1 buf2 store1 store2 <->
+        interp_store_rel (brimpl l r) v buf1 buf2 store1 store2.
   Proof.
     split; intros; destruct l, r; unfold brimpl in *;
     autorewrite with interp_store_rel in *; auto; intuition.
@@ -549,7 +487,7 @@ Section ConfRel.
     fun x y =>
       interp_conf_state phi.(cr_st) x y ->
       forall valu,
-        interp_store_rel phi.(cr_rel) valu x y.
+        interp_store_rel phi.(cr_rel) valu x.(conf_buf) y.(conf_buf) x.(conf_store) y.(conf_store).
 
   Definition crel :=
     list (conf_rel).
@@ -577,8 +515,8 @@ Section ConfRel.
     { e_prem: crel;
       e_concl: conf_rel }.
 
-  Definition interp_entailment (i: relation conf) (e: entailment) : relation conf :=
-    fun q1 q2 =>
+  Definition interp_entailment (i: relation conf) (e: entailment) :=
+    forall q1 q2,
       interp_crel i e.(e_prem) q1 q2 ->
       interp_conf_rel e.(e_concl) q1 q2.
 
@@ -591,7 +529,7 @@ Section ConfRel.
     (buf2: n_tuple bool b2)
     store1 store2
   :=
-    forall valu, interp_simplified_store_rel (projT2 scr) valu buf1 buf2 store1 store2.
+    forall valu, interp_store_rel (projT2 scr) valu buf1 buf2 store1 store2.
 
   Definition simplify_conf_rel (cr: conf_rel) :=
     existT _ cr.(cr_ctx) cr.(cr_rel).
@@ -606,12 +544,7 @@ Section ConfRel.
                                   c1.(conf_store)
                                   c2.(conf_store)).
   Proof.
-    unfold interp_simplified_conf_rel, interp_conf_rel.
-    intuition.
-    - apply interp_store_rel_simplify.
-      now unfold simplify_conf_rel.
-    - apply interp_store_rel_simplify.
-      apply H2.
+    now unfold interp_simplified_conf_rel, interp_conf_rel.
   Qed.
 
   Definition simplified_crel := list simplified_conf_rel.
@@ -683,9 +616,15 @@ Section ConfRel.
       se_concl: simplified_conf_rel; }.
 
   Definition interp_simplified_entailment
+    (i: relation state_template)
     (se: simplified_entailment)
   :=
-    forall (buf1: n_tuple bool se.(se_st).(cs_st1).(st_buf_len)) (buf2: n_tuple bool se.(se_st).(cs_st2).(st_buf_len)) store1 store2,
+    state_template_sane se.(se_st).(cs_st1) ->
+    state_template_sane se.(se_st).(cs_st2) ->
+    i se.(se_st).(cs_st1) se.(se_st).(cs_st2) ->
+    forall (buf1: n_tuple bool se.(se_st).(cs_st1).(st_buf_len))
+           (buf2: n_tuple bool se.(se_st).(cs_st2).(st_buf_len))
+           (store1 store2: store (P4A.interp a)),
       interp_simplified_crel se.(se_prems) buf1 buf2 store1 store2 ->
       interp_simplified_conf_rel se.(se_concl) buf1 buf2 store1 store2.
 
@@ -695,15 +634,10 @@ Section ConfRel.
        se_concl := simplify_conf_rel e.(e_concl); |}.
 
   Lemma simplify_entailment_correct (e: entailment):
-    e.(e_concl).(cr_st).(cs_st1).(st_buf_len) <
-      size' (P4A.interp a) e.(e_concl).(cr_st).(cs_st1).(st_state) ->
-    e.(e_concl).(cr_st).(cs_st2).(st_buf_len) <
-      size' (P4A.interp a) e.(e_concl).(cr_st).(cs_st2).(st_state) ->
     forall i: Relations.rel state_template,
-      (forall q1 q2, interp_entailment (fun c1 c2 => i (conf_to_state_template c1)
-                                                       (conf_to_state_template c2)) e q1 q2) <->
-      (i e.(e_concl).(cr_st).(cs_st1) e.(e_concl).(cr_st).(cs_st2) ->
-       interp_simplified_entailment (simplify_entailment e)).
+      interp_entailment (fun c1 c2 => i (conf_to_state_template c1)
+                                        (conf_to_state_template c2)) e <->
+      interp_simplified_entailment i (simplify_entailment e).
   Proof.
     intros.
     unfold interp_entailment, simplify_entailment, interp_simplified_entailment; simpl.
@@ -711,57 +645,53 @@ Section ConfRel.
     - pose (q1 := {|
         conf_state := e.(e_concl).(cr_st).(cs_st1).(st_state);
         conf_store := store1;
-        conf_buf_sane := H0;
+        conf_buf_sane := H1;
         conf_buf := buf1;
       |}).
       pose (q2 := {|
         conf_state := e.(e_concl).(cr_st).(cs_st2).(st_state);
         conf_store := store2;
-        conf_buf_sane := H1;
+        conf_buf_sane := H2;
         conf_buf := buf2;
       |}).
       replace buf1 with (conf_buf q1) by reflexivity.
       replace buf2 with (conf_buf q2) by reflexivity.
       replace store1 with (conf_store q1) by reflexivity.
       replace store2 with (conf_store q2) by reflexivity.
-      apply simplify_conf_rel_correct with (c1 := q1) (c2 := q2).
-      + apply H2; auto.
+      apply simplify_conf_rel_correct with (c1 := q1) (c2 := q2); subst q1 q2.
+      + apply H0; auto.
         eapply simplify_crel_correct; try split.
-        * subst q1 q2.
-          unfold interp_state_template; simpl.
-          intuition.
-        * subst q1 q2.
-          unfold interp_state_template; simpl.
-          intuition.
-        * unfold conf_to_state_template.
-          subst q1 q2.
-          simpl.
-          destruct (e.(e_concl).(cr_st).(cs_st1)).
-          destruct (e.(e_concl).(cr_st).(cs_st2)).
-          now simpl.
+        * now unfold interp_state_template; simpl.
+        * now unfold interp_state_template; simpl.
+        * unfold conf_to_state_template; simpl.
+          now (destruct (e.(e_concl).(cr_st).(cs_st1));
+               destruct (e.(e_concl).(cr_st).(cs_st2))).
         * apply H4.
-      + subst q1 q2.
-        unfold interp_conf_state, interp_state_template; simpl.
-        intuition.
+      + now unfold interp_conf_state, interp_state_template; simpl.
     - apply simplify_conf_rel_correct; intros.
-      unfold interp_conf_state, interp_state_template in H4.
-      destruct H4 as [[? ?] [? ?]].
-      rewrite H5, H7 in H2.
-      apply H2; auto.
-      * clear H2.
+      destruct H2 as [[? ?] [? ?]].
+      rewrite H3, H5 in H0.
+      apply H0; auto.
+      * unfold state_template_sane.
+        rewrite H3, H2.
+        apply q1.
+      * unfold state_template_sane.
+        rewrite H4, H5.
+        apply q2.
+      * clear H0.
         induction (e_prem e).
-        + cbn in H3.
-          unfold conf_to_state_template in H3.
-          rewrite <- H4, <- H5, <- H6, <- H7 in H3.
+        + cbn in H1.
+          unfold conf_to_state_template in H1.
+          rewrite <- H2, <- H3, <- H4, <- H5 in H1.
           destruct (cs_st1 (cr_st (e_concl e))).
           destruct (cs_st2 (cr_st (e_concl e))).
           now simpl in *.
-        + rewrite interp_crel_cons in H3.
+        + rewrite interp_crel_cons in H1.
           apply IHc.
           intuition.
       * eapply simplify_crel_correct; auto.
         + now unfold interp_conf_state, interp_state_template.
-        + exact H3.
+        + exact H1.
   Qed.
 End ConfRel.
 Arguments interp_conf_rel {_} {_} {_} {_} {_} _.
